prove aes_iv_put

investigations/bedrock2/Aes/Aes.v
@@ -23,6 +23,11 @@ Section Impl.
   Local Notation "2" := (expr.literal 2) (in custom bedrock_expr).
   Local Notation "3" := (expr.literal 3) (in custom bedrock_expr).
   Local Notation "4" := (expr.literal 4) (in custom bedrock_expr).
+  Local Notation "5" := (expr.literal 5) (in custom bedrock_expr).
+  Local Notation "6" := (expr.literal 6) (in custom bedrock_expr).
+  Local Notation "7" := (expr.literal 7) (in custom bedrock_expr).
+  Local Notation "8" := (expr.literal 8) (in custom bedrock_expr).
+  Local Notation "9" := (expr.literal 9) (in custom bedrock_expr).
 
   (**** aes.c
     void aes_init(aes_cfg_t aes_cfg) {
@@ -54,44 +59,56 @@ Section Impl.
 
   (**** aes.c
     void aes_key_put(const void *key, aes_key_len_t key_len) {
-  // Determine how many key registers to use.
-  size_t num_regs_key_used;
-  if (key_len == kAes256) {
-    num_regs_key_used = 8;
-  } else if (key_len == kAes192) {
-    num_regs_key_used = 6;
-  } else {
-    num_regs_key_used = 4;
-  }
+      // Determine how many key registers to use.
+      size_t num_regs_key_used;
+      if (key_len == kAes256) {
+        num_regs_key_used = 8;
+      } else if (key_len == kAes192) {
+        num_regs_key_used = 6;
+      } else {
+        num_regs_key_used = 4;
+      }
 
-  // Write the used key registers.
-  for (int i = 0; i < num_regs_key_used; ++i) {
-    REG32(AES_KEY0(0) + i * sizeof(uint32_t)) = ((uint32_t * )key)[i];
-  }
-  // Write the unused key registers (the AES unit requires all key registers to
-  // be written).
-  for (int i = num_regs_key_used; i < AES_NUM_REGS_KEY; ++i) {
-    REG32(AES_KEY0(0) + i * sizeof(uint32_t)) = 0x0;
-  }
+      // Write the used key registers.
+      for (int i = 0; i < num_regs_key_used; ++i) {
+        REG32(AES_KEY0(0) + i * sizeof(uint32_t)) = ((uint32_t * )key)[i];
+      }
+      // Write the unused key registers (the AES unit requires all key registers to
+      // be written).
+      for (int i = num_regs_key_used; i < AES_NUM_REGS_KEY; ++i) {
+        REG32(AES_KEY0(0) + i * sizeof(uint32_t)) = 0x0;
+      }
     }
    ***)
-  (* TODO: put the enums in constants and use them!
-  (* N.B. the bedrock2 version avoids the aes_key_len_t enum by taking the key
-     length as a word *)
   Definition aes_key_put : func :=
     let key := "key" in
     let key_len := "key_len" in
-    let num_regs_key_used := "num_regs_key_used" inb
+    let num_regs_key_used := "num_regs_key_used" in
     let i := "i" in
     ("b2_iv_put",
-     (globals ++ [key; key_len], [], bedrock_func_body:(
-      
+     (aes_globals ++ [key; key_len], [], bedrock_func_body:(
+      if (key_len == kAes256) {
+        num_regs_key_used = 8
+      } else {
+        if (key_len == kAes192) {
+          num_regs_key_used = 6
+        } else {
+          num_regs_key_used = 4
+        }
+      };
+
       i = 0 ;
-      while (i < AES_NUM_REGS_IV) {
-        output! WRITE (AES_IV0 + i * 4, load4( iv + i ));
+      while (i < num_regs_key_used) {
+        output! WRITE (AES_KEY0 + i * 4, load4(key + i ));
+        i = i + 1
+      };
+
+      i = num_regs_key_used ;
+      while (i < AES_NUM_REGS_KEY) {
+        output! WRITE (AES_KEY0 + i * 4, 0);
         i = i + 1
       }
-    ))). *)
+    ))).
 
   (**** aes.c
     void aes_iv_put(const void *iv) {
@@ -101,14 +118,21 @@ Section Impl.
       }
     }
    ***)
+  (* N.B. *)
   Definition aes_iv_put : func :=
     let iv := "iv" in
     let i := "i" in
     ("b2_iv_put",
      (aes_globals ++ [iv], [], bedrock_func_body:(
       i = 0 ;
+                                                    (*
+      output! WRITE (AES_IV0, load4( iv ));
+      output! WRITE (AES_IV0 + 4, load4( iv + 1 ));
+      output! WRITE (AES_IV0 + 8, load4( iv + 2 ));
+      output! WRITE (AES_IV0 + 12, load4( iv + 3 ))
+      *)
       while (i < AES_NUM_REGS_IV) {
-        output! WRITE (AES_IV0 + i * 4, load4( iv + i ));
+        output! WRITE (AES_IV0 + (i * 4), load4( iv + (i * 4) ));
         i = i + 1
       }
     ))).
