investigations/bedrock2/Aes/AesProperties.v
@@ -2,7 +2,11 @@ Require Import Coq.Strings.String.
 Require Import Coq.Lists.List.
 Require Import Coq.micromega.Lia.
 Require Import Coq.ZArith.ZArith.
+Require Import bedrock2.Array.
+Require Import bedrock2.Map.Separation.
+Require Import bedrock2.Map.SeparationLogic.
 Require Import bedrock2.ProgramLogic.
+Require Import bedrock2.Scalars.
 Require Import bedrock2.Semantics.
 Require Import bedrock2.Syntax.
 Require Import bedrock2.TailRecursion.
@@ -12,6 +16,7 @@ Require Import coqutil.Word.Interface.
 Require Import coqutil.Word.Properties.
 Require Import coqutil.Map.Interface.
 Require Import coqutil.Tactics.Tactics.
+Require Import coqutil.Tactics.syntactic_unify.
 Require Import coqutil.Tactics.letexists.
 Require Import Cava.Util.Tactics.
 Require Import Bedrock2Experiments.StateMachineSemantics.
@@ -33,19 +38,42 @@ Section Proofs.
 
   (***** General-purpose lemmas/tactics and setup *****)
 
-  Add Ring wring : (Properties.word.ring_theory (word := Semantics.word))
+  Add Ring wring : (Properties.word.ring_theory (word := parameters.word))
         (preprocess [autorewrite with rew_word_morphism],
-         morphism (Properties.word.ring_morph (word := Semantics.word)),
+         morphism (Properties.word.ring_morph (word := parameters.word)),
          constants [Properties.word_cst]).
 
   Existing Instance constant_names | 10.
 
+  (* This tactic simplifies implicit types so that they all agree; otherwise
+     tactic has trouble connecting, for instance, a word of type parameters.word
+     and a word of type Semantics.word, even though they are the same *)
+  Local Ltac simplify_implicits :=
+    change Semantics.word with parameters.word in *;
+    change Semantics.mem with parameters.mem in *;
+    change Semantics.width with 32 in *;
+    change Semantics.word_ok with parameters.word_ok in *;
+    change Semantics.mem_ok with parameters.mem_ok in *.
+
+  Local Ltac invert_step :=
+    lazymatch goal with
+    | H : step _ _ _ _ _ |- _ => inversion H; clear H; subst
+    end.
+
+  Lemma execution_step action args rets t s s':
+    execution t s -> step action s args rets s' ->
+    execution ((map.empty, action, args, (map.empty, rets)) :: t) s'.
+  Proof. intros; cbn [execution]; eauto. Qed.
+  Lemma invert1_execution action args rets t s':
+    execution ((map.empty, action, args, (map.empty, rets)) :: t) s' ->
+    exists s, execution t s /\ step action s args rets s'.
+  Proof. intros; cbn [execution]; eauto. Qed.
+
   Lemma interact_mmio call action binds arges t m l
         (post : trace -> mem -> locals -> Prop) (args : list Semantics.word) :
     dexprs m l arges args ->
-    (forall s s' (rets : list Semantics.word),
-        execution t s ->
-        step action s args rets s' ->
+    (forall s' (rets : list Semantics.word),
+        execution ((map.empty, action, args, (map.empty, rets)) :: t) s' ->
         (exists l0 : locals,
             map.putmany_of_list_zip binds rets l = Some l0 /\
             post ((map.empty, action, args, (map.empty, rets)) :: t) m l0)) ->
@@ -60,23 +88,73 @@ Section Proofs.
   Qed.
 
   Local Ltac interaction :=
-    eapply interact_mmio; [ solve [repeat straightline_with_map_lookup] | ];
-    repeat straightline;
+    (* get trace *)
+    let t := lazymatch goal with
+             | |- cmd _ (cmd.interact _ _ _) ?t _ _ _ => t end in
+    eapply interact_mmio;
+    [ solve [repeat straightline_with_map_lookup;
+             simplify_implicits; repeat straightline_with_map_lookup] | ];
+    simplify_implicits; intros;
     lazymatch goal with
-    | H : step _ _ _ _ _ |- _ => inversion H; clear H; subst
+    | H : execution (_ :: t) _ |- _ =>
+      pose proof H; apply invert1_execution in H; destruct H as [? [? ?]]
+    end; invert_step; repeat straightline.
+
+  Fixpoint repeat_logic_step
+           (logic : Semantics.trace -> Semantics.mem -> Semantics.locals ->
+                    (Semantics.trace -> Semantics.mem -> Semantics.locals -> Prop) -> Prop)
+           (n : nat) post : Semantics.trace -> Semantics.mem -> locals -> Prop :=
+    match n with
+    | O => post
+    | S n => fun t m l => logic t m l (repeat_logic_step logic n post)
     end.
+
+  Lemma unroll_while functions conde body t m l
+        (iterations : nat)
+        (post : trace -> mem -> locals -> Prop) (cond : Semantics.word) :
+    repeat_logic_step
+      (fun t m l post =>
+         exists cond,
+           dexpr m l conde cond
+           /\ word.unsigned cond <> 0
+           /\ cmd (call functions) body t m l post)
+      iterations (fun t m l =>
+                    dexpr m l conde cond
+                    /\ word.unsigned cond = 0
+                    /\ post t m l) t m l ->
+    cmd (call functions) (cmd.while conde body) t m l post.
+  Proof.
+    lazymatch goal with
+      |- repeat_logic_step ?logic _ ?post _ _ _ -> _ =>
+      set (step:=logic);
+        set (P:=post)
+    end.
+    intros. exists nat, lt, (fun i => repeat_logic_step step i P).
+    ssplit.
+    { exact lt_wf. }
+    { eauto. }
+    { intro i. destruct i; cbn [repeat_logic_step].
+      { (* i=0 case (contradiction) *)
+        subst P. repeat straightline.
+        eexists; ssplit; eauto; congruence. }
+      { (* i <> 0 case *)
+        subst step. repeat straightline.
+        eexists; ssplit; eauto; try congruence; [ ].
+        repeat straightline.
+        eapply Proper_cmd; [ apply Proper_call | | eassumption ].
+        repeat intro. exists i. ssplit; eauto. } }
+  Qed.
 
   Hint Extern 4 (step _ ?s _ _ _) =>
   eapply (ReadStep (p:=state_machine_parameters) s) : step.
   Hint Extern 4 (step _ ?s _ _ _) =>
   eapply (WriteStep (p:=state_machine_parameters) s) : step.
-  Hint Constructors read_step : step.
-  Hint Constructors write_step : step.
+
+  Lemma word_add_0_r (w : parameters.word) : word.add w (word.of_Z 0) = w.
+  Proof. ring. Qed.
 
   Lemma reg_addr_unique r1 r2 : reg_addr r1 = reg_addr r2 -> r1 = r2.
   Proof.
-    assert (forall w, word.add w (word.of_Z 0) = w) as word_add_0
-        by (intros; ring).
     pose proof addrs_unique as Huniq.
     cbv [aes_reg_addrs list_reg_addrs] in *.
     rewrite nregs_key_eq, nregs_iv_eq, nregs_data_eq in Huniq.
@@ -88,7 +166,7 @@ Section Proofs.
            | _ => progress cbn [seq map app] in Huniq
            end.
     simplify_unique_words_in Huniq.
-    rewrite !word_add_0 in *. clear word_add_0.
+    rewrite !word_add_0_r in *.
     cbv [reg_addr]; cbn; intro Heqaddr.
     destruct r1.
     (* clear all hypothesis that don't have to do with r1 (makes proof
@@ -110,6 +188,23 @@ Section Proofs.
     all:destruct r2; try first [ exact eq_refl | congruence ].
   Qed.
 
+  (* run [interaction] and then assert the register's identity *)
+  Local Ltac interaction_with_reg R :=
+    (* this simplification step ensures that the parameters.reg_addr hypothesis
+       we see is a new one *)
+    cbn [parameters.reg_addr parameters.write_step parameters.read_step
+                             state_machine_parameters] in *;
+    interaction;
+    lazymatch goal with
+    | H : parameters.reg_addr ?r = ?addr |- _ =>
+      replace addr with (reg_addr R) in H
+        by (cbn [reg_addr]; subst_lets; ring);
+      apply reg_addr_unique in H; try subst r
+    end;
+    (* simplify again *)
+    cbn [parameters.reg_addr parameters.write_step parameters.read_step
+                             state_machine_parameters] in *.
+
   Lemma execution_unique (t : trace) s1 s2 :
     execution t s1 ->
     execution t s2 ->
@@ -125,37 +220,59 @@ Section Proofs.
     | H1 : execution t ?s1, H2 : execution t ?s2 |- _ =>
       specialize (IHt _ _ H1 H2); subst
     end.
-    repeat (lazymatch goal with
-            | x := _ |- _ => subst x
-            | |- ?x = ?x => reflexivity
-            | H : is_busy (BUSY _ _ _) = false |- _ =>
-              cbv [is_busy] in H; exfalso; congruence
-            | H : parameters.reg_addr _ = reg_addr _ |- _ =>
-              apply reg_addr_unique in H; subst
-            | H : step _ _ _ _ _ |- _ =>
-              inversion H; clear H; subst
-            | H : parameters.read_step _ _ _ _ |- _ =>
-              inversion H; clear H; subst
-            | H : parameters.write_step _ _ _ _ |- _ =>
-              inversion H; clear H; subst
-            | _ => first [ invert_bool
-                        | progress cbn [status_matches_state
-                                          is_input_reg
-                                          is_output_reg] in *]
-            end; try congruence).
+    repeat invert_step;
+      cbn [parameters.read_step parameters.write_step
+                                state_machine_parameters] in *;
+      cbv [read_step write_step] in *.
+    all: repeat lazymatch goal with
+                | H : False |- _ => contradiction H
+                | H : _ /\ _ |- _ => destruct H
+                | H : _ = reg_addr _ |- _ => apply reg_addr_unique in H; subst
+                | |- ?x = ?x => reflexivity
+                | _ => first [ progress subst
+                            | destruct_one_match_hyp ]
+                end.
   Qed.
 
   Local Ltac infer_states_equal :=
-    repeat match goal with
+    repeat lazymatch goal with
            | H1 : execution ?t _, H2 : execution ?t _ |- _ =>
              pose proof execution_unique _ _ _ H1 H2; subst;
              clear H2; one_goal_or_solved ltac:(try congruence)
            end.
 
-  Lemma execution_step action args rets t s s':
-    execution t s -> step action s args rets s' ->
-    execution ((map.empty, action, args, (map.empty, rets)) :: t) s'.
-  Proof. intros; cbn [execution]; eauto. Qed.
+  Lemma ControlReg_is_CTRL r : reg_category r = ControlReg -> r = CTRL.
+  Proof. destruct r; cbn [reg_category]; congruence. Qed.
+
+  Local Ltac infer_registers_equal :=
+    repeat lazymatch goal with
+           | H : reg_category _ = ControlReg |- _ =>
+             apply ControlReg_is_CTRL in H; subst
+           end.
+
+  Local Ltac infer_state_data_equal :=
+    repeat lazymatch goal with
+           | H : IDLE _ = IDLE _ |- _ => inversion H; clear H; subst
+           | H : BUSY _ _ _ = BUSY _ _ _ |- _ => inversion H; clear H; subst
+           | H : DONE _ = DONE _ |- _ => inversion H; clear H; subst
+           end.
+
+  Local Ltac invert_write_step_nobranch :=
+    lazymatch goal with
+    | H : write_step _ _ _ _ |- _ =>
+      cbv [write_step] in H; cbn [reg_category] in H
+    end;
+    repeat lazymatch goal with
+           | H : False |- _ => contradiction H
+           | _ => destruct_one_match_hyp
+           end; [ ].
+
+  Local Ltac infer :=
+    repeat first [ progress infer_registers_equal
+                 | progress infer_states_equal
+                 | progress infer_state_data_equal
+                 | progress invert_write_step_nobranch
+                 | progress invert_step ].
 
   Local Notation aes_op_t := (enum_member aes_op) (only parsing).
   Local Notation aes_mode_t := (enum_member aes_mode) (only parsing).
@@ -169,6 +286,9 @@ Section Proofs.
     select_bits ctrl AES_CTRL_KEY_LEN_OFFSET AES_CTRL_KEY_LEN_MASK.
   Definition ctrl_manual_operation (ctrl : parameters.word) : bool :=
     is_flag_set ctrl AES_CTRL_MANUAL_OPERATION.
+
+  (* prevent [inversion] from exposing word.of_Z in constants *)
+  Local Opaque constant_words.
 
   (***** Proofs for specific functions *****)
 
@@ -197,7 +317,7 @@ Section Proofs.
                    register value and no other known register values *)
                 (exists ctrl,
                     execution tr' (IDLE (map.put (map:=parameters.regs)
-                                                 map.empty (AES_CTRL : Semantics.word) ctrl))
+                                                 map.empty AES_CTRL ctrl))
                     /\ ctrl_operation ctrl = word.eqb aes_cfg_operation (word.of_Z 0)
                     /\ ctrl_mode ctrl = aes_cfg_mode
                     /\ ctrl_key_len ctrl = aes_cfg_key_len
@@ -208,8 +328,6 @@ Section Proofs.
                 (* ...and there is no output *)
                 /\ rets = []).
 
-  (* prevent [inversion] from exposing word.of_Z in constants *)
-  Opaque constant_words.
 
   Lemma aes_init_correct :
     program_logic_goal_for_function! aes_init.
@@ -219,7 +337,6 @@ Section Proofs.
 
     (* write CTRL *)
     interaction.
-    repeat straightline.
 
     (* done; prove postcondition *)
     ssplit; auto; [ ].
@@ -239,24 +356,18 @@ Section Proofs.
            end.
 
     (* infer information from the last step *)
-    infer_states_equal.
     cbn [parameters.write_step state_machine_parameters] in *.
-    lazymatch goal with
-    | H : write_step _ ?r ?v _ |- _ =>
-      inversion H; subst
-    end; [ ].
+    infer.
 
-    (* make sure implicit types all agree *)
-    change Semantics.word with parameters.word in *.
-    change Semantics.width with 32 in *.
-    change Semantics.word_ok with parameters.word_ok in *.
+    simplify_implicits.
 
     (* split cases *)
     eexists; ssplit.
     { (* prove that the execution trace is OK *)
-      eapply execution_step; eauto with step. }
+      eapply execution_step; eauto; [ ].
+      econstructor; eauto; reflexivity. }
     { (* prove that the "operation" flag is correct *)
-      cbv [ctrl_operation]. clear H11.
+      cbv [ctrl_operation].
       rewrite !is_flag_set_or_shiftl_low by lia.
       apply is_flag_set_shift; eauto using size1_boolean.
       lia. }
@@ -271,5 +382,92 @@ Section Proofs.
     { cbv [ctrl_manual_operation].
       apply is_flag_set_or_shiftl_high;
         (eassumption || prove_has_size || lia). }
+  Qed.
+
+  Instance spec_of_aes_iv_put : spec_of aes_iv_put :=
+    fun function_env =>
+      forall (tr : trace) (m : mem) R
+        (rs : known_register_state)
+        (iv_ptr iv0 iv1 iv2 iv3 : Semantics.word),
+        (* iv array is in memory *)
+        (array scalar32 (word.of_Z 4) iv_ptr [iv0;iv1;iv2;iv3] * R)%sep m ->
+        (* circuit must be in IDLE state *)
+        execution tr (IDLE rs) ->
+        let args := [iv_ptr] in
+        call function_env aes_iv_put tr m (aes_globals ++ args)
+             (fun tr' m' rets =>
+                (* the circuit is in IDLE state with the iv registers updated *)
+                execution tr'
+                          (IDLE (map.put
+                                   (map.put
+                                      (map.put
+                                         (map.put rs (reg_addr IV0) iv0)
+                                         (reg_addr IV1) iv1)
+                                      (reg_addr IV2) iv2)
+                                   (reg_addr IV3) iv3))
+                (* ...and the same properties as before hold on the memory *)
+                /\ (array scalar32 (word.of_Z 4) iv_ptr [iv0;iv1;iv2;iv3] * R)%sep m'
+                (* ...and there is no output *)
+                /\ rets = []).
+
+  Lemma aes_iv_put_correct :
+    program_logic_goal_for_function! aes_iv_put.
+  Proof.
+    (* initial processing *)
+    repeat straightline.
+    simplify_implicits.
+
+    (* simplify array predicate *)
+    cbn [array] in *.
+    repeat match goal with
+           | H : context [scalar32 ?addr] |- _ =>
+             progress ring_simplify addr in H
+           end.
+
+    (* this assertion helps prove that i does not get truncated *)
+    assert (4 < 2 ^ Semantics.width) by (cbn; lia).
+
+    (* unroll while loop *)
+    eapply unroll_while with (iterations:=4%nat). cbn [repeat_logic_step].
+    repeat straightline.
+
+    (* process each iteration of the while loop *)
+
+    (* i = 0 *)
+    split; repeat straightline.
+    { subst_lets. simplify_implicits. push_unsigned.
+      rewrite nregs_iv_eq. destruct_one_match; lia. }
+    interaction_with_reg IV0. infer; subst.
+
+    (* i = 1 *)
+    split; repeat straightline.
+    { subst_lets. simplify_implicits. push_unsigned.
+      rewrite nregs_iv_eq. destruct_one_match; lia. }
+    interaction_with_reg IV1. infer; subst.
+
+    (* i = 2 *)
+    split; repeat straightline.
+    { subst_lets. simplify_implicits. push_unsigned.
+      rewrite nregs_iv_eq. destruct_one_match; lia. }
+    interaction_with_reg IV2. infer; subst.
+
+    (* i = 3 *)
+    split; repeat straightline.
+    { subst_lets. simplify_implicits. push_unsigned.
+      rewrite nregs_iv_eq. destruct_one_match; lia. }
+    interaction_with_reg IV3. infer; subst.
+
+    (* i = 4; loop done *)
+    ssplit; repeat straightline; [ | ].
+    { subst_lets. simplify_implicits. push_unsigned.
+      rewrite nregs_iv_eq. destruct_one_match; lia. }
+
+    (* done; prove postcondition *)
+    cbn [array].
+    repeat match goal with
+           | |- context [scalar32 ?addr] =>
+             progress ring_simplify addr
+           end.
+    ssplit; eauto.
   Qed.
 End Proofs.
